
\ifind
\section*{Example question}
\else
\subsection*{5 binomial distribution - example question}
\fi
Show the variance of the binomial distribution is $npq$.

\noindent \textbf{solution}
This is a hard question. As ever we start with
\begin{equation}
1=Z=\sum_{r=0}^n \left(\begin{array}{c} n\\r\end{array}\right) p^rq^{n-r}
\end{equation}
and we take the second derivative
\begin{eqnarray}
\frac{d^2Z}{dp^2}&=&\sum_{r=0}^n \left(\begin{array}{c} n\\r\end{array}\right) r(r-1)p^{r-2}q^{n-r}-2\sum_{r=0}^n \left(\begin{array}{c} n\\r\end{array}\right) r(n-r)p^{r-1}q^{n-r-1}\cr&&+\sum_{r=0}^n \left(\begin{array}{c} n\\r\end{array}\right)(n-r)(n-r-1) p^rq^{n-r-2}
\end{eqnarray}
so
\begin{equation}
0=\sum_{r=0}^n\left[\frac{1}{p^2}(r^2-r)-\frac{2}{pq}(rn-r^2)+\frac{1}{q^2}(n^2-2nr-n+r^2+r)\right]\left(\begin{array}{c} n\\r\end{array}\right) p^rq^{n-r}
\end{equation}
or, using $\langle R\rangle = np$,
\begin{equation}
0=\frac{1}{p^2}\langle R^2\rangle - \frac{1}{p^2}np-\frac{2n}{pq}np+\frac{2}{pq}\langle R^2\rangle +(n^2-n)\frac{1}{q^2}-(2n-1)\frac{1}{q^2}np+\frac{1}{q^2}\langle R^2\rangle
\end{equation}
Putting this together we get
\begin{equation}
0=\left(\frac{1}{p}+\frac{1}{q}\right)^2\langle R^2\rangle - \frac{n}{p}-\frac{2n^2}{q}+ \frac{n^2-n}{q^2}-\frac{(2n^2-n)p}{q^2}
\end{equation}
Simplifying we get
\begin{equation}
0=\frac{\langle R^2\rangle}{p^2q^2}-\frac{n^2}{q^2}-\frac{n}{p}-\frac{n}{q}
\end{equation}
so
\begin{equation}
\langle R^2\rangle=n^2p^2+npq
\end{equation}
and finally
\begin{equation}
\sigma^2=\langle R^2\rangle-\langle R\rangle^2=npq
\end{equation}



